isabelle/ABT.thy
@@ -1,0 +1,109 @@
+theory ABT
+  imports Main
+begin
+
+type_synonym var = nat
+
+datatype 'op ABT =
+  Var var
+  | App 'op "('op Arg) list"
+and 'op Arg =
+  Trm "'op ABT"
+| Bnd "'op Arg"
+
+type_synonym 'v sub = "var \<Rightarrow> 'v"
+
+fun cons_aux :: "'v \<Rightarrow> 'v sub \<Rightarrow> 'v sub" where
+  "(cons_aux v \<sigma>) 0 = v" |
+  "(cons_aux v \<sigma>) (Suc x) = \<sigma> x"
+
+definition cons :: "'v \<Rightarrow> 'v sub \<Rightarrow> 'v sub" (infixl "\<bullet>" 55) where
+  "v \<bullet> \<sigma> \<equiv> cons_aux v \<sigma>"
+
+(********************** locale substable ***************************)
+locale substable =
+  fixes trm :: "'op ABT" (* just for purposes of talking about 'op *)
+  and shift :: "'v \<Rightarrow> 'v" ("\<Up>")
+  and var2val :: "var \<Rightarrow>'v" ("\<lfloor>_\<rfloor>")
+  and quote :: "'v \<Rightarrow> 'op ABT"
+  assumes var2val_lift: "\<lfloor>Suc x\<rfloor> \<equiv> \<Up> \<lfloor>x\<rfloor>"
+begin
+
+  abbreviation lift_sub :: "'v sub \<Rightarrow> 'v sub" ("\<Up>") where
+    "\<Up> \<sigma> x \<equiv> \<Up> (\<sigma> x)"
+  
+  abbreviation ext :: "'v sub \<Rightarrow> 'v sub" where
+    "ext \<sigma> \<equiv> \<lfloor>0\<rfloor> \<bullet> (\<Up> \<sigma>)"
+  
+  fun map_abt :: "'v sub \<Rightarrow> 'op ABT \<Rightarrow> 'op ABT" ("\<llangle>_\<rrangle>_" 70)
+    and map_arg :: "'v sub \<Rightarrow> 'op Arg \<Rightarrow> 'op Arg" ("\<llangle>_\<rrangle>\<^sub>a_" 70)
+    where
+   "\<llangle>\<sigma>\<rrangle> (Var x) = quote (\<sigma> x)" |
+   "\<llangle>\<sigma>\<rrangle> (App op args) = App op (map (map_arg \<sigma>) args)" |
+   "\<llangle>\<sigma>\<rrangle>\<^sub>a (Trm M) = Trm (\<llangle>\<sigma>\<rrangle> M)" |
+   map_arg_bnd:"\<llangle>\<sigma>\<rrangle>\<^sub>a (Bnd A) = Bnd (\<llangle>ext \<sigma>\<rrangle>\<^sub>a A)" 
+
+end
+
+(********************** locale substable2 **************************************)
+locale substable2 = L: substable trm s v2v q + R: substable trm s' v2v' q'
+    for trm and s and v2v and q and s' and q' and v2v'
+begin
+  
+  abbreviation cong :: "'b sub \<Rightarrow> 'c sub \<Rightarrow> bool" (infixl "\<cong>" 30) where
+    "\<sigma> \<cong> \<tau> \<equiv> \<forall> x. q (\<sigma> x) =  q' (\<tau> x)"
+  
+  abbreviation map_cong_P1 :: "'a ABT \<Rightarrow> bool" where
+    "map_cong_P1 M \<equiv> \<forall> \<sigma> \<tau>. \<sigma> \<cong> \<tau> \<longrightarrow> (\<forall> \<sigma> \<tau>. \<sigma> \<cong> \<tau> \<longrightarrow> L.ext \<sigma> \<cong> R.ext \<tau> )
+            \<longrightarrow> L.map_abt \<sigma> M = R.map_abt \<tau> M"
+  
+  abbreviation map_cong_P2 :: "'a Arg \<Rightarrow> bool" where
+    "map_cong_P2 A \<equiv> \<forall> \<sigma> \<tau>. \<sigma> \<cong> \<tau> \<longrightarrow> (\<forall> \<sigma> \<tau>. \<sigma> \<cong> \<tau> \<longrightarrow> L.ext \<sigma> \<cong> R.ext \<tau> )
+            \<longrightarrow> L.map_arg \<sigma> A = R.map_arg \<tau> A"
+  
+  lemma map_cong_aux: "map_cong_P1 M"
+    by (induction M rule: ABT.induct[of map_cong_P1 map_cong_P2]) 
+       (auto simp add: L.map_arg_bnd R.map_arg_bnd)
+  
+  theorem map_cong: assumes 1: "\<sigma> \<cong> \<tau>" and 2: "\<And> \<sigma> \<tau>. \<sigma> \<cong> \<tau> \<Longrightarrow> L.ext \<sigma> \<cong> R.ext \<tau>"
+    shows "L.map_abt \<sigma> M = R.map_abt \<tau> M"
+    using 1 2 map_cong_aux[of M] by blast
+
+end
+
+(********************** locale substable3 **************************************)
+locale substable3 = S1: substable trm s1 v2v1 q1 + S2: substable trm s2 v2v2 q2
+    + S3: substable trm s3 v2v3 q3
+    for trm and s1 and v2v1 and q1 and s2 and q2 and v2v2 and s3 and q3 and v2v3
+begin
+  
+  (*   (\<sigma> ; \<tau>) = \<rho>    *)
+  abbreviation comp_cong :: "'c sub \<Rightarrow> 'b sub \<Rightarrow> 'd sub \<Rightarrow> bool" where
+    "comp_cong \<tau> \<sigma> \<rho> \<equiv> \<forall> x. S2.map_abt \<tau> (q1 (\<sigma> x)) = q3 (\<rho> x)"
+  
+  abbreviation map_fusion_P1 :: "'a ABT \<Rightarrow> bool" where
+    "map_fusion_P1 M \<equiv> \<forall> \<sigma> \<tau> \<rho>. comp_cong \<tau> \<sigma> \<rho> 
+          \<longrightarrow> S2.map_abt \<tau> (S1.map_abt \<sigma> M) = S3.map_abt \<rho> M"
+  abbreviation map_fusion_P2 :: "'a Arg \<Rightarrow> bool" where
+    "map_fusion_P2 M \<equiv> \<forall> \<sigma> \<tau> \<rho>. comp_cong \<tau> \<sigma> \<rho> 
+          \<longrightarrow> S2.map_arg \<tau> (S1.map_arg \<sigma> M) = S3.map_arg \<rho> M"
+  
+  lemma map_fusion_aux: 
+    assumes 1: "\<forall> \<sigma> \<tau> \<rho>. comp_cong \<tau> \<sigma> \<rho> \<longrightarrow> comp_cong (S2.ext \<tau>) (S1.ext \<sigma>) (S3.ext \<rho>)"
+    shows "map_fusion_P1 M"
+    apply (induction M rule: ABT.induct[of map_fusion_P1 map_fusion_P2])
+    apply force
+      apply force
+     apply force
+    apply simp apply clarify using 1 apply fast
+    done
+  
+  theorem map_fusion:
+    assumes 1: "comp_cong \<tau> \<sigma> \<rho>"
+    and 2: "\<forall> \<sigma> \<tau> \<rho>. comp_cong \<tau> \<sigma> \<rho> \<longrightarrow> comp_cong (S2.ext \<tau>) (S1.ext \<sigma>) (S3.ext \<rho>)"
+    shows "S2.map_abt \<tau> (S1.map_abt \<sigma> M) = S3.map_abt \<rho> M"
+    using map_fusion_aux 1 2 by fast
+
+end
+
+end
