isabelle/Rename.thy
@@ -1,0 +1,123 @@
+theory Rename
+  imports Main ABT
+begin
+
+interpretation var_s: substable "Var 0" "Suc" "\<lambda> x. x" "Var"
+  by unfold_locales auto
+
+definition extr :: "var sub \<Rightarrow> var sub" where
+  "extr \<rho> \<equiv> var_s.ext \<rho>"
+
+definition rename :: "var sub \<Rightarrow> 'op ABT \<Rightarrow> 'op ABT" where
+  "rename \<equiv> var_s.map_abt"
+
+definition seqrr :: "var sub \<Rightarrow> var sub \<Rightarrow> var sub" (infixl "r;r" 70) where
+  "(\<sigma> r;r \<rho>) x \<equiv> \<rho> (\<sigma> x)"
+
+lemma extr_cons_seq[simp]: "extr \<rho> = 0 \<bullet> (\<rho> r;r Suc)"
+  unfolding extr_def seqrr_def by simp
+
+theorem RIdL[simp]: "(\<lambda> x. x) r;r \<rho> = \<rho>"
+  unfolding seqrr_def by simp
+
+theorem RShiftId[simp]: "Suc r;r (\<lambda> x. x) = Suc"
+  unfolding seqrr_def by simp
+
+theorem RHeadCons[simp]: "(x \<bullet> \<rho>) 0 = x"
+  unfolding cons_def by simp
+
+theorem RTailCons[simp]: "(y \<bullet> \<sigma>) (Suc x) = \<sigma> x"
+  unfolding cons_def by simp 
+
+theorem RShiftCons[simp]: "Suc r;r (x \<bullet> \<rho>) = \<rho>"
+  unfolding cons_def  seqrr_def shift_def by simp
+
+(********************** locale subst_quote_shift ***************************)
+locale subst_quote_shift = substable +
+  assumes quote_var: "quote \<lfloor>x\<rfloor> = Var x"
+  and quote_shift: "quote (\<Up> v) = rename Suc (quote v)"
+begin
+  
+  lemma id_ext: "(\<forall> x. quote (\<sigma> x) = Var x) \<Longrightarrow> quote ((ext \<sigma>) x) = Var x"
+    apply (case_tac x)
+    using quote_var apply (force simp add: cons_def)
+    using quote_shift apply (force simp add: cons_def rename_def)
+    done
+  
+  abbreviation P_id_abt :: "'a ABT \<Rightarrow> bool" where
+    "P_id_abt M \<equiv> \<forall> \<sigma>. (\<forall> x. quote (\<sigma> x) = Var x)
+       \<longrightarrow> map_abt \<sigma> M = M"
+  abbreviation P_id_arg :: "'a Arg \<Rightarrow> bool" where
+    "P_id_arg A \<equiv> \<forall> \<sigma>. (\<forall> x. quote (\<sigma> x) = Var x)
+        \<longrightarrow> map_arg \<sigma> A = A"
+  
+  lemma map_id_aux: "P_id_abt M"
+    apply (induction M rule: ABT.induct[of P_id_abt P_id_arg])
+       apply force
+      apply simp apply clarify apply (rule map_idI) apply blast
+     apply force
+    apply simp apply clarify using id_ext apply force
+    done
+  
+  theorem map_abt_id: 
+    assumes 1: "\<And> x. quote (\<sigma> x) = Var x"
+    shows "map_abt \<sigma> M = M" using 1 map_id_aux by fast
+
+end
+(********************** end subst_quote_shift ***************************)
+
+interpretation var_sqs: subst_quote_shift "Var 0" Suc "\<lambda> x. x" Var
+  by unfold_locales (auto simp: rename_def)
+  
+theorem rename_id[simp]: "rename (\<lambda> x. x) M = M"
+  unfolding rename_def by (rule var_sqs.map_abt_id) simp
+
+theorem RIdR[simp]: "\<rho> r;r (\<lambda> x. x) = \<rho>"
+  unfolding seqrr_def by (rule ext) simp
+
+theorem RConsSeq[simp]: "(y \<bullet> \<sigma>) r;r \<tau> =  (\<tau> y) \<bullet> (\<sigma> r;r \<tau>)"
+  apply (rule ext)
+  apply (case_tac x)
+  unfolding seqrr_def apply simp 
+  apply simp
+  done
+
+theorem RAssoc[simp]: "(\<rho> r;r \<sigma>) r;r \<tau> = \<rho> r;r (\<sigma> r;r \<tau>)"
+  unfolding seqrr_def by simp
+
+interpretation rrr: 
+  substable3 "Var 0" Suc "\<lambda> x. x" Var Suc Var "\<lambda> x. x" Suc Var "\<lambda> x. x"
+  by unfold_locales 
+
+lemma rrr_comp_cong_ext: assumes 1: "\<sigma> r;r \<tau> = \<rho>"
+  shows "extr \<sigma> r;r extr \<tau> = extr \<rho>"
+proof simp
+  have            "0 \<bullet> \<sigma> r;r (\<tau> r;r Suc) 
+                 = 0 \<bullet> (\<sigma> r;r \<tau>) r;r Suc" by simp
+  also have "... = 0 \<bullet> \<rho> r;r Suc" using 1 by simp
+  finally show "0 \<bullet> \<sigma> r;r (\<tau> r;r Suc) = 0 \<bullet> \<rho> r;r Suc" .
+qed
+
+theorem rename_fusion:
+  assumes 1: "\<forall> x. \<sigma> (\<rho> x) = \<tau> x"
+  shows "rename \<sigma> (rename \<rho> M) = rename \<tau> M"
+  unfolding rename_def 
+proof (rule rrr.map_fusion)
+  show " \<forall>x. var_s.map_abt \<sigma> (Var (\<rho> x)) = Var (\<tau> x)"
+    using 1 apply force done
+next
+  show " \<forall>\<sigma> \<tau> \<rho>.
+       (\<forall>x. var_s.map_abt \<tau> (Var (\<sigma> x)) = Var (\<rho> x)) \<longrightarrow>
+       (\<forall>x. var_s.map_abt (var_s.ext \<tau>) (Var (var_s.ext \<sigma> x)) = Var (var_s.ext \<rho> x))"
+  proof clarify
+    fix \<sigma> :: "var sub" and \<tau> \<rho> x
+    assume "\<forall>x. var_s.map_abt \<tau> (Var (\<sigma> x)) = Var (\<rho> x)"
+    then have "\<sigma> r;r \<tau> = \<rho>" unfolding seqrr_def by simp
+    then have "extr \<sigma> r;r extr \<tau> = extr \<rho>" by (rule rrr_comp_cong_ext)
+    then have "(extr \<sigma> r;r extr \<tau>) x = (extr \<rho>) x" by simp
+    then show "var_s.map_abt (var_s.ext \<tau>) (Var (var_s.ext \<sigma> x)) = Var (var_s.ext \<rho> x)"
+      unfolding seqrr_def extr_def by simp
+  qed
+qed
+
+end
